proofs/fstar/models/Ark_ec.Hashing.Curve_maps.Wb.fst
@@ -1,1 +1,3 @@
 module Ark_ec.Hashing.Curve_maps.Wb
+
+assume new type t_WBMap (config : Type0) : Type0
