proofs/fstar/models/Ark_r1cs_std.Alloc.fst
@@ -1,1 +1,5 @@
 module Ark_r1cs_std.Alloc
+
+open Rust_primitives
+assume val f_new_input : #f:Type0 -> #v:Type0 -> Ark_relations.R1cs.Constraint_system.t_ConstraintSystemRef f -> unit -> Core_models.Result.t_Result v Ark_relations.R1cs.Error.t_SynthesisError
+assume val f_new_witness : #f:Type0 -> #v:Type0 -> Ark_relations.R1cs.Constraint_system.t_ConstraintSystemRef f -> unit -> Core_models.Result.t_Result v Ark_relations.R1cs.Error.t_SynthesisError
