proofs/fstar/models/Ark_r1cs_std.Eq.fst
@@ -1,1 +1,3 @@
 module Ark_r1cs_std.Eq
+
+assume val f_enforce_equal : #a:Type0 -> #b:Type0 -> a -> b -> Core_models.Result.t_Result unit Ark_relations.R1cs.Error.t_SynthesisError
