proofs/fstar/models/Ark_r1cs_std.Fields.Emulated_fp.Field_var.fst
@@ -1,1 +1,3 @@
 module Ark_r1cs_std.Fields.Emulated_fp.Field_var
+
+assume new type t_EmulatedFpVar (target : Type0) (base : Type0) : Type0
