proofs/fstar/models/Ark_r1cs_std.Fields.Fp.fst
@@ -1,1 +1,3 @@
 module Ark_r1cs_std.Fields.Fp
+
+assume new type t_FpVar (f : Type0) : Type0
