proofs/fstar/models/Ark_r1cs_std.R1cs_var.fst
@@ -1,1 +1,3 @@
 module Ark_r1cs_std.R1cs_var
+
+assume val f_value : #a:Type0 -> a -> Core_models.Result.t_Result a Ark_relations.R1cs.Error.t_SynthesisError
