proofs/fstar/models/Ark_relations.R1cs.Constraint_system.fst
@@ -16,3 +16,15 @@ assume val impl_7__set_mode : #f:Type0 -> Ark_relations.R1cs.Constraint_system.t
 type t_SynthesisMode =
   | SynthesisMode_Prove : t_SynthesisMode
   | SynthesisMode_Setup : t_SynthesisMode
+
+assume val f_generate_constraints : #f:Type0 -> #c:Type0 -> c -> t_ConstraintSystemRef f -> Core_models.Result.t_Result unit Ark_relations.R1cs.Error.t_SynthesisError
+
+assume val impl_7__finalize : #f:Type0 -> t_ConstraintSystemRef f -> unit
+
+assume val impl_7__is_satisfied : #f:Type0 -> Ark_relations.R1cs.Constraint_system.t_ConstraintSystemRef f -> Core_models.Result.t_Result bool Ark_relations.R1cs.Error.t_SynthesisError
+
+assume val impl_7__num_instance_variables : #f:Type0 -> Ark_relations.R1cs.Constraint_system.t_ConstraintSystemRef f -> Rust_primitives.Integers.usize
+assume val impl_7__num_witness_variables : #f:Type0 -> Ark_relations.R1cs.Constraint_system.t_ConstraintSystemRef f -> Rust_primitives.Integers.usize
+assume val impl_7__num_constraints : #f:Type0 -> Ark_relations.R1cs.Constraint_system.t_ConstraintSystemRef f -> Rust_primitives.Integers.usize
+
+assume val impl_7__to_matrices : #f:Type0 -> t_ConstraintSystemRef f -> Core_models.Result.t_Result (t_ConstraintMatrices f) Ark_relations.R1cs.Error.t_SynthesisError
