proofs/fstar/models/Num_traits.Identities.fst
@@ -1,3 +1,5 @@
 module Num_traits.Identities
 
 assume val f_zero : #t:Type0 -> unit -> t
+
+assume val f_is_zero : #t:Type0 -> t -> bool
